theories/L6_PCPS/Heap/compat.v
@@ -7,80 +7,550 @@ From Coq Require Import NArith.BinNat Relations.Relations MSets.MSets
                         MSets.MSetRBT Lists.List omega.Omega Sets.Ensembles.
 From L6 Require Import functions cps ctx eval cps_util identifiers ctx Ensembles_util
      List_util Heap.heap Heap.heap_defs Heap.space_sem Heap.closure_conversion
-     Heap.cc_log_rel tactics.
+     Heap.cc_log_rel tactics Heap.size_cps set_util.
 From compcert Require Import lib.Coqlib.
 
 Import ListNotations.
 
-
-
 Module Compat (H : Heap).
+
+  Module S := Size H.
   
-  Module LR := CC_log_rel H.
-
-  Import H LR LR.Sem LR.Sem.Equiv LR.Sem.Equiv.Defs.
-    (** Conditions *)
-
-  Section LR_Preds.
+  Import H S S.LR S.LR.Sem S.LR.Sem.Equiv S.LR.Sem.Equiv.Defs S.LR.Sem.Equiv.Defs.HL.
+  
+  Section CompatDefs.
+    
+    Variable (clo_tag : cTag).
 
     Context (IG : GInv) (* Final global *)
-            (ILi : nat -> Inv) (* Final local indexed by a natural number indicating the amount of time units already spent for evaluation of the RHS program *) 
+            (IL1 IL2: Inv) (* Final local *)
+
             (IIG : GIInv) (* Global initial *)
             (IIL1 IIL2 : IInv) (* Local initial *)
-            (F : nat). (* A constant factor*)
+
+            (M : nat) (* memory cost factor *)
+            (F : nat) (* time cost factor *).
 
 
-    (** Compatibility properties for local invariants to do local reasoning *)
-
-    Context
-      (InvCostTimeout :
-         forall (H1 H2 : heap block) (rho1 rho2 : env) (e1 e2 : exp) (k c : nat),
-           IIL1 (H1, rho1, e1) (H2, rho2, e2) ->
-           ILi k (c, size_heap H1) (c - k, size_heap H2)).
-    
-    Context
-      (InvCostBase :
-         forall (H1 H2 : heap block) (rho1 rho2 : env) (e1 e2 : exp) (k c : nat),
-           c >= 1 ->
-           IIL1 (H1, rho1, e1) (H2, rho2, e2) ->
-           ILi k (c, size_heap H1) (c, size_heap H2)).
-    
-    
-    (** * Compatibility properties for local conditions *)
+    (** * Global precondition respects heap equivalence  *)
 
     Context
-      (InvCompat_str :
-         forall (k1 k2 c1 c2 c1' c2' m1 m2 : nat),
+      (IInvGC :
+         forall (H1 H1' H2 H2' : heap block) (rho1 rho2 : env) (e1 e2 : exp),
+           IIG (H1, rho1, e1) (H2, rho2, e2) ->
+           live (env_locs rho1 (occurs_free e1)) H1 H1' ->
+           live' (env_locs rho2 (occurs_free e2)) H2 H2' ->
+           IIG (H1', rho1, e1) (H2', rho2, e2)).
+ 
+
+    (** * Global postcondition respects heap equivalence  *)
+
+    Context
+      (InvHeapEquiv :
+         forall (H1 H1' H2 H2' : heap block) (rho1 rho2 rho1' rho2': env) (e1 e2 : exp)
+           (c1 c2 : nat) (m1 m2 : nat) k β1 β2,
+           IG k (H1', rho1', e1, c1, m1) (H2', rho2', e2, c2, m2) ->
+
+           (occurs_free e1) |- (H1, rho1) ⩪_(id, β1) (H1', rho1') ->
+           injective_subdomain (reach' H1' (env_locs rho1' (occurs_free e1))) β1 ->
+
+           (occurs_free e2) |- (H2, rho2) ⩪_(β2, id) (H2', rho2') ->
+           injective_subdomain (reach' H2 (env_locs rho2 (occurs_free e2))) β2 ->
+                              
+           IG k (H1, rho1, e1, c1, m1) (H2, rho2, e2, c2, m2)
+      ).
+
+    Context
+      (InvHeapEquiv' :
+         forall (H1 H1' H2 H2' : heap block) (rho1 rho2 rho1' rho2': env) (e1 e2 : exp)
+           (c1 c2 : nat) (m1 m2 : nat) k β1 β2,
+           IG k (H1, rho1, e1, c1, m1) (H2, rho2, e2, c2, m2) ->
+
+           (occurs_free e1) |- (H1, rho1) ⩪_(id, β1) (H1', rho1') ->
+           injective_subdomain (reach' H1' (env_locs rho1' (occurs_free e1))) β1 ->
+
+           (occurs_free e2) |- (H2, rho2) ⩪_(β2, id) (H2', rho2') ->
+           injective_subdomain (reach' H2 (env_locs rho2 (occurs_free e2))) β2 ->
+                              
+            IG k (H1', rho1', e1, c1, m1) (H2', rho2', e2, c2, m2)
+      ).
+
+    Lemma InvGC :
+      forall (H1 H1' H2 H2' : heap block) (rho1 rho2 : env) (e1 e2 : exp)
+        (c1 c2 : nat) (m1 m2 : nat) k,
+        IG k (H1', rho1, e1, c1, m1) (H2', rho2, e2, c2, m2) ->
+        
+        live (env_locs rho1 (occurs_free e1)) H1 H1' ->
+        live' (env_locs rho2 (occurs_free e2)) H2 H2' ->
+                              
+        IG k (H1, rho1, e1, c1, m1) (H2, rho2, e2, c2, m2).
+    Proof. 
+      intros ? ? ? ? ? ? ? ? ? ? ? ? ? ? Hgc1 Hgc2.
+      destruct Hgc1 as (? & ? & ? & ?); destruct Hgc2 as (? & ? & ? & ?).
+      eapply InvHeapEquiv; eauto.
+      eapply heap_env_equiv_heap_equiv; eauto.
+      eapply heap_env_equiv_heap_equiv; eauto.
+    Qed.
+
+
+    (* Context *)
+    (*   (LInvHeapEquiv : *)
+    (*      forall (H1 H1' H2 H2' : heap block) (rho1 rho2 rho1' rho2': env) (e1 e2 : exp) *)
+    (*        (c1 c2 : nat) (m1 m2 : nat) k β1 β2, *)
+    (*        IL k (H1', rho1', e1, c1, m1) (H2', rho2', e2, c2, m2) -> *)
+
+    (*        (occurs_free e1) |- (H1, rho1) ⩪_(id, β1) (H1', rho1') -> *)
+    (*        injective_subdomain (reach' H1' (env_locs rho1' (occurs_free e1))) β1 -> *)
+
+    (*        (occurs_free e2) |- (H2, rho2) ⩪_(β2, id) (H2', rho2') -> *)
+    (*        injective_subdomain (reach' H2 (env_locs rho2 (occurs_free e2))) β2 -> *)
+                              
+    (*        IL k (H1, rho1, e1, c1, m1) (H2, rho2, e2, c2, m2) *)
+    (*   ). *)
+
+    (* Context *)
+    (*   (LInvHeapEquiv' : *)
+    (*      forall (H1 H1' H2 H2' : heap block) (rho1 rho2 rho1' rho2': env) (e1 e2 : exp) *)
+    (*        (c1 c2 : nat) (m1 m2 : nat) k β1 β2, *)
+    (*        IL k (H1, rho1, e1, c1, m1) (H2, rho2, e2, c2, m2) -> *)
+
+    (*        (occurs_free e1) |- (H1, rho1) ⩪_(id, β1) (H1', rho1') -> *)
+    (*        injective_subdomain (reach' H1' (env_locs rho1' (occurs_free e1))) β1 -> *)
            
-           ILi k2 (c1 - c1', m1) (c2 - c2', m2) -> 
+    (*        (occurs_free e2) |- (H2, rho2) ⩪_(β2, id) (H2', rho2') -> *)
+    (*        injective_subdomain (reach' H2 (env_locs rho2 (occurs_free e2))) β2 -> *)
+                              
+    (*        IL k (H1', rho1', e1, c1, m1) (H2', rho2', e2, c2, m2) *)
+    (*   ). *)
 
-           c1' <= c2' + (k1 - k2) <= c1' + F*c1' ->
+    (* Lemma LInvGC : *)
+    (*   forall (H1 H1' H2 H2' : heap block) (rho1 rho2 : env) (e1 e2 : exp) *)
+    (*     (c1 c2 : nat) (m1 m2 : nat) k, *)
+    (*     IL k (H1', rho1, e1, c1, m1) (H2', rho2, e2, c2, m2) -> *)
+        
+    (*     live (env_locs rho1 (occurs_free e1)) H1 H1' -> *)
+    (*     live' (env_locs rho2 (occurs_free e2)) H2 H2' -> *)
+                              
+    (*     IL k (H1, rho1, e1, c1, m1) (H2, rho2, e2, c2, m2). *)
+    (* Proof.  *)
+    (*   intros ? ? ? ? ? ? ? ? ? ? ? ? ? ? Hgc1 Hgc2. *)
+    (*   destruct Hgc1 as (? & ? & ? & ?); destruct Hgc2 as (? & ? & ? & ?). *)
+    (*   eapply LInvHeapEquiv; eauto. *)
+    (*   eapply heap_env_equiv_heap_equiv; eauto. *)
+    (*   eapply heap_env_equiv_heap_equiv; eauto. *)
+    (* Qed. *)
 
-           ILi k1 (c1, m1) (c2, m2)).
+    (** * Base case and timout compatibility *)
+
+    Definition InvCostBase (H1 H2 : heap block) (rho1 rho2 : env) (e1 e2 : exp) :=
+      forall (H1' H2' : heap block) (rho1' rho2' : env) (c : nat) β1 β2,
+        (occurs_free e1) |- (H1, rho1) ⩪_(id, β1) (H1', rho1') ->
+        injective_subdomain (reach' H1' (env_locs rho1' (occurs_free e1))) β1 ->
+           
+        (occurs_free e2) |- (H2, rho2) ⩪_(β2, id) (H2', rho2') ->
+        injective_subdomain (reach' H2 (env_locs rho2 (occurs_free e2))) β2 ->
+                           
+        IIL1 (H1', rho1', e1) (H2', rho2', e2) ->
+                           
+        IL1 (H1', rho1', e1, c, size_heap H1') (H2', rho2', e2, c, size_heap H2').
+
+    (** * Constructor application compatibility *) 
+
+    Definition InvCtxCompat (H1 H2 : heap block) (rho1 rho2 : env) (C1 C2 : exp_ctx) (e1 e2 : exp)  :=
+      forall (H1' H2' H1'' H2'' : heap block) (rho1' rho2' rho1'' rho2'' : env) c1 c2 c1' c2' m1 m2  β1 β2,
+        (occurs_free (C1 |[ e1 ]|)) |- (H1, rho1) ⩪_(id, β1) (H1', rho1') ->
+        injective_subdomain (reach' H1' (env_locs rho1' (occurs_free (C1 |[ e1 ]|)))) β1 ->
+           
+        (occurs_free (C2 |[ e2 ]|)) |- (H2, rho2) ⩪_(β2, id) (H2', rho2') ->
+        injective_subdomain (reach' H2 (env_locs rho2 (occurs_free (C2 |[ e2 ]|)))) β2 ->
+
+        IL2 (H1'', rho1'', e1, c1 - c1', m1) (H2'', rho2'', e2, c2 - c2', m2) ->
+        
+        ctx_to_heap_env C1 H1' rho1' H1'' rho1'' c1' ->
+        ctx_to_heap_env_CC C2 H2' rho2' H2'' rho2'' c2' ->
+        
+        IL1 (H1', rho1', C1 |[ e1 ]|, c1, m1) (H2', rho2', C2 |[ e2 ]|, c2, m2).
     
+    Definition IInvCtxCompat (H1 H2 : heap block) (rho1 rho2 : env) (C1 C2 : exp_ctx) (e1 e2 : exp)  :=
+      forall (H1' H2' H1'' H2'' : heap block) (rho1' rho2' rho1'' rho2'' : env) c1' c2' β1 β2,
+        (occurs_free (C1 |[ e1 ]|)) |- (H1, rho1) ⩪_(id, β1) (H1', rho1') ->
+        injective_subdomain (reach' H1' (env_locs rho1' (occurs_free (C1 |[ e1 ]|)))) β1 ->
+           
+        (occurs_free (C2 |[ e2 ]|)) |- (H2, rho2) ⩪_(β2, id) (H2', rho2') ->
+        injective_subdomain (reach' H2 (env_locs rho2 (occurs_free (C2 |[ e2 ]|)))) β2 ->                           
+
+        IIL1 (H1', rho1', C1 |[ e1 ]|) (H2', rho2', C2 |[ e2 ]|) ->
+            
+        ctx_to_heap_env C1 H1' rho1' H1'' rho1'' c1' ->
+        ctx_to_heap_env_CC C2 H2' rho2' H2'' rho2'' c2' ->
+
+        IIL2 (H1'', rho1'', e1) (H2'', rho2'', e2).
+
+    Definition InvCtxCompat_r (H1 H2 : heap block) (rho1 rho2 : env) (C : exp_ctx) (e1 e2 : exp) :=
+      forall (H1' H2' H1'' H2'' : heap block) (rho1' rho2' rho1'' rho2'' : env) c' c1 c2 m1 m2 β1 β2,
+        (occurs_free e1) |- (H1, rho1) ⩪_(id, β1) (H1', rho1') ->
+        injective_subdomain (reach' H1' (env_locs rho1' (occurs_free e1))) β1 ->
+           
+        (occurs_free (C |[ e2 ]|)) |- (H2, rho2) ⩪_(β2, id) (H2', rho2') ->
+        injective_subdomain (reach' H2 (env_locs rho2 (occurs_free (C |[ e2 ]|)))) β2 ->
+                                      
+        IL2 (H1'', rho1'', e1, c1, m1) (H2'', rho2'', e2, c2 - c', m2) ->
+        
+        ctx_to_heap_env_CC C H2' rho2' H2'' rho2'' c' ->
+        
+        IL1 (H1', rho1', e1, c1, m1) (H2', rho2', C |[ e2 ]|, c2, m2).
+
+    Definition IInvCtxCompat_r (H1 H2 : heap block) (rho1 rho2 : env) (C : exp_ctx) (e1 e2 : exp) :=
+      forall (H1' H2' H1'' H2'' : heap block) (rho1' rho2' rho1'' rho2'' : env) c' β1 β2,
+        (occurs_free e1) |- (H1, rho1) ⩪_(id, β1) (H1', rho1') ->
+        injective_subdomain (reach' H1' (env_locs rho1' (occurs_free e1))) β1 ->
+           
+        (occurs_free (C |[ e2 ]|)) |- (H2, rho2) ⩪_(β2, id) (H2', rho2') ->
+        injective_subdomain (reach' H2 (env_locs rho2 (occurs_free (C |[ e2 ]|)))) β2 ->
+                                   
+        IIL1 (H1', rho1', e1) (H2', rho2', C |[ e2 ]|) ->
+            
+        ctx_to_heap_env_CC C H2' rho2' H2'' rho2'' c' ->
+
+        IIL2 (H1'', rho1'', e1) (H2'', rho2'', e2).
+
+
+    (** * Case compatibility *)
+    
+    Definition IInvCaseHdCompat (H1 H2 : heap block) (rho1 rho2 : env) x1 x2 t Pats1 Pats2 (e1 e2 : exp) :=
+      (forall H1' rho1' H2' rho2' β1 β2,
+         (occurs_free (Ecase x1 ((t, e1) :: Pats1))) |- (H1, rho1) ⩪_(id, β1) (H1', rho1') ->
+         injective_subdomain (reach' H1' (env_locs rho1' (occurs_free (Ecase x1 ((t, e1) :: Pats1))))) β1 ->
+           
+         (occurs_free (Ecase x2 ((t, e2) :: Pats2))) |- (H2, rho2) ⩪_(β2, id) (H2', rho2') ->
+         injective_subdomain (reach' H2 (env_locs rho2 (occurs_free (Ecase x2 ((t, e2) :: Pats2))))) β2 ->
+
+         IIL1 (H1', rho1', Ecase x1 ((t, e1) :: Pats1)) (H2', rho2', Ecase x2 ((t, e2) :: Pats2)) ->
+         IIL2 (H1', rho1', e1) (H2', rho2', e2)).
+
+      Definition IInvCaseTlCompat (H1 H2 : heap block) (rho1 rho2 : env)  x1 x2 t Pats1 Pats2 (e1 e2 : exp) :=
+        (forall H1' rho1' H2' rho2' β1 β2,
+         (occurs_free (Ecase x1 ((t, e1) :: Pats1))) |- (H1, rho1) ⩪_(id, β1) (H1', rho1') ->
+         injective_subdomain (reach' H1' (env_locs rho1' (occurs_free (Ecase x1 ((t, e1) :: Pats1))))) β1 ->
+           
+         (occurs_free (Ecase x2 ((t, e2) :: Pats2))) |- (H2, rho2) ⩪_(β2, id) (H2', rho2') ->
+         injective_subdomain (reach' H2 (env_locs rho2 (occurs_free (Ecase x2 ((t, e2) :: Pats2))))) β2 ->
+                                                       
+         IIL1 (H1', rho1', Ecase x1 ((t, e1) :: Pats1)) (H2', rho2', Ecase x2 ((t, e2) :: Pats2)) ->
+         IIL1 (H1', rho1', Ecase x1 Pats1) (H2', rho2', Ecase x2 Pats2)).
+
+      Definition InvCaseHdCompat (H1 H2 : heap block) (rho1 rho2 : env) x1 x2 t Pats1 Pats2 (e1 e2 : exp) :=
+        (forall H1' rho1' H2' rho2' β1 β2 c1 c2 m1 m2,
+           (occurs_free (Ecase x1 ((t, e1) :: Pats1))) |- (H1, rho1) ⩪_(id, β1) (H1', rho1') ->
+           injective_subdomain (reach' H1' (env_locs rho1' (occurs_free (Ecase x1 ((t, e1) :: Pats1))))) β1 ->
+           
+           (occurs_free (Ecase x2 ((t, e2) :: Pats2))) |- (H2, rho2) ⩪_(β2, id) (H2', rho2') ->
+           injective_subdomain (reach' H2 (env_locs rho2 (occurs_free (Ecase x2 ((t, e2) :: Pats2))))) β2 ->
+
+           IL2 (H1', rho1', e1, c1 - cost (Ecase x1 ((t, e1) :: Pats1)), m1) (H2', rho2', e2, c2 - cost (Ecase x2 ((t, e2) :: Pats2)), m2)  ->
+           IL1 (H1', rho1', Ecase x1 ((t, e1) :: Pats1), c1, m1) (H2', rho2', Ecase x2 ((t, e2) :: Pats2), c2, m2)).
+
+      Definition InvCaseTlCompat (H1 H2 : heap block) (rho1 rho2 : env) x1 x2 t Pats1 Pats2 (e1 e2 : exp) :=
+        (forall H1' rho1' H2' rho2' β1 β2 c1 c2 m1 m2,
+           (occurs_free (Ecase x1 ((t, e1) :: Pats1))) |- (H1, rho1) ⩪_(id, β1) (H1', rho1') ->
+           injective_subdomain (reach' H1' (env_locs rho1' (occurs_free (Ecase x1 ((t, e1) :: Pats1))))) β1 ->
+           
+           (occurs_free (Ecase x2 ((t, e2) :: Pats2))) |- (H2, rho2) ⩪_(β2, id) (H2', rho2') ->
+           injective_subdomain (reach' H2 (env_locs rho2 (occurs_free (Ecase x2 ((t, e2) :: Pats2))))) β2 ->
+
+           IL1 (H1', rho1', Ecase x1 Pats1, c1, m1) (H2', rho2', Ecase x2 Pats2, c2, m2) ->
+           IL1 (H1', rho1', Ecase x1 ((t, e1) :: Pats1), c1, m1) (H2', rho2', Ecase x2 ((t, e2) :: Pats2), c2, m2)).
+     
+    (** * App compatibility *)
+    
+    Definition IInvAppCompat (H1 H2 : heap block) (rho1 rho2 : env) f1 t xs1 f2 xs2 f2' Γ :=   
+      forall (i  : nat) (H1' H2' : heap block)
+        (rho_clo rho_clo1 rho_clo2 rho2' : env)
+        (B1 : fundefs) (f1' : var) (ct1 : cTag)
+        (xs1' : list var) (e1 : exp) (l1 env_loc1 : loc)
+        (vs1 : list value) 
+        (B2 : fundefs) (f3 : var) (c ct2 : cTag) (xs2' : list var) 
+        (e2 : exp) (l2 env_loc2 : loc) (vs2 : list value) c1 c2 m1 m2,
+        
+        IG i (H1', rho_clo2, e1, c1, m1) (H2', rho2', e2, c2, m2) ->
+        IIG (H1', rho_clo2, e1) (H2', rho2', e2) ->
+        
+        M.get f1 rho1 = Some (Loc l1) ->
+        get l1 H1 = Some (Clos (FunPtr B1 f1') (Loc env_loc1)) ->
+        get env_loc1 H1 = Some (Env rho_clo) ->
+        find_def f1' B1 = Some (ct1, xs1', e1) ->
+        getlist xs1 rho1 = Some vs1 ->
+        def_closures B1 B1 rho_clo H1 env_loc1 = (H1', rho_clo1) ->
+        setlist xs1' vs1 rho_clo1 = Some rho_clo2 ->
+        
+        
+        M.get f2 rho2 = Some (Loc l2) ->
+        getlist xs2 rho2 = Some vs2 ->
+        get l2 H2 = Some (Constr c [FunPtr B2 f3; Loc env_loc2]) ->
+        Some rho2' =
+        setlist xs2' (Loc env_loc2 :: vs2) (def_funs B2 B2 (M.empty value)) ->
+        find_def f3 B2 = Some (ct2, xs2', e2) ->
+        
+        IL1 (H1, rho1, Eapp f1 t xs1, c1 + cost (Eapp f1 t xs1), max m1 (size_heap H1'))
+           (H2, rho2, AppClo clo_tag f2 t xs2 f2' Γ, c2 + 1 + 1 + cost (Eapp f2' t (Γ :: xs2)), max m2 (size_heap H2')).
+    
+  End CompatDefs.
+
+  Section CompatLemmas.
+    
+    Variable (clo_tag : cTag).
+
+    Context (IG : GInv) (* Final global *)
+            (IL1 IL2: Inv) (* Final local *)
+
+            (IIG : GIInv) (* Global initial *)
+            (IIL1 IIL2 : IInv). (* Local initial *)
+
+    (* TODO move *)
+    Lemma live_deterministic S (_ : set_util.ToMSet S) H1 H2 H2' :
+      live S H1 H2 ->
+      live S H1 H2' ->
+      (exists b1 b2, S |- H2 ≃_(b1, b2) H2' /\
+      injective_subdomain (reach' H2 S) b1 /\
+      injective_subdomain (reach' H2' S) b2).
+    Proof.
+      intros [Hyp1 [b1 [Hyp2 Hinj1]]] [Hyp1' [b2 [Hyp2' Hinj2]]].
+      eexists b1, b2. symmetry in Hyp2. 
+      rewrite <- (Combinators.compose_id_right _ _ id) in Hyp2.
+      rewrite <- (Combinators.compose_id_left _ _ b2).
+      split; [| split ]; eauto.
+      eapply heap_equiv_f_compose; [| eassumption ]. eassumption.
+    Qed.
+
     Context
-      (InvTransfer :
-         forall (k c1 c2 c m1 m2 : nat),
-           ILi (k + c) (c1, m1) (c2, m2) ->
-           ILi k (c1, m1) (c2 + c, m2)).
+      (IInvGC :
+         forall (H1 H1' H2 H2' : heap block) (rho1 rho2 : env) (e1 e2 : exp),
+           IIG (H1, rho1, e1) (H2, rho2, e2) ->
+           live (env_locs rho1 (occurs_free e1)) H1 H1' ->
+           live' (env_locs rho2 (occurs_free e2)) H2 H2' ->
+           IIG (H1', rho1, e1) (H2', rho2, e2)).
+        
+    (** Application compatibility *)
+    Lemma cc_approx_exp_app_compat (k j : nat) (b : Inj) (H1 H2 : heap block)
+          (rho1 rho2 : env) (f1 : var) (xs1 : list var)
+          (f2 f2' Γ : var) (xs2 : list var) (t : fTag) :
+      IInvAppCompat clo_tag IG IL1 IIG H1 H2 rho1 rho2 f1 t xs1 f2 xs2 f2' Γ ->
+      InvCostBase IL1 IIL1 H1 H2 rho1 rho2 (Eapp f1 t xs1) (AppClo clo_tag f2 t xs2 f2' Γ) ->
+
+      well_formed (reach' H1 (env_locs rho1 (occurs_free (Eapp f1 t xs1)))) H1 ->
+      well_formed (reach' H2 (env_locs rho2 (occurs_free (AppClo clo_tag f2 t xs2 f2' Γ)))) H2 ->
+      (env_locs rho1 (occurs_free (Eapp f1 t xs1))) \subset dom H1 ->
+      (env_locs rho2 (occurs_free (AppClo clo_tag f2 t xs2 f2' Γ))) \subset dom H2 ->
+      
+      ~ Γ \in (f2 |: FromList xs2) ->
+      ~ f2' \in (f2 |: FromList xs2) ->
+      Γ <> f2' ->
+                
+      cc_approx_var_env k j IIG IG b H1 rho1 H2 rho2 f1 f2 ->
+      Forall2 (cc_approx_var_env k j IIG IG b H1 rho1 H2 rho2) xs1 xs2 ->
+
+      (Eapp f1 t xs1, rho1, H1) ⪯ ^ (k ; j; IIL1 ; IIG
+                                     ; IL1
+                                     ; IG)
+      (AppClo clo_tag f2 t xs2 f2' Γ, rho2, H2).
+    Proof with now eauto with Ensembles_DB.
+      intros Hiinv Hbase Hwf1 Hwf2 Hs1 Hs2 Hnin1 Hnin2 Hneq  Hvar Hall
+             b1 b2 H1' H2' rho1' rho2' v1 c1 m1 Heq1 Hinj1 Heq2 Hinj2
+             HII Hleq1 Hstep1 Hstuck1.
+      eapply (cc_approx_var_env_heap_env_equiv
+                _ _ 
+                (occurs_free (Eapp f1 t xs1))
+                (occurs_free (AppClo clo_tag f2 t xs2 f2' Γ))) in Hvar;
+          [| eassumption | eassumption | eassumption | eassumption 
+           | normalize_occurs_free; now eauto with Ensembles_DB
+           | unfold AppClo; normalize_occurs_free; now eauto with Ensembles_DB ].
+      inv Hstep1. 
+      (* Timeout! *)
+      - { edestruct (Hstuck1 (cost (Eapp f1 t xs1))) as [v1 [m1 Hstep1]].
+          inv Hstep1; [ omega | ].
+          exists OOT, c1. destruct (lt_dec c1 1).
+          - eexists. eexists id. repeat split. now constructor; eauto.
+            now eapply injective_subdomain_Empty_set. rewrite <- plus_n_O.
+            eapply Hbase; try eassumption.
+            now rewrite cc_approx_val_eq.
+          - edestruct Hvar as [l2 [Hget' Hcc]]; eauto.
+            simpl in Hcc. rewrite Hgetl in Hcc. destruct l2 as [l2 | ]; [| contradiction ].
+            destruct (get l2 H2') as [v |] eqn:Hget2; try contradiction.
+            destruct Hcc as [Hbeq Hcc]; subst; simpl in Hcc.
+            destruct v as [ ? [| [| B2 f3 ] [| [ env_loc' |] [|] ]] | | ]; try contradiction.
+            destruct Hcc as [Him Hcc].
+            edestruct Hcc with (vs2 := vs) as (xs2' & e2 & rho2'' & Hfind' & Hset' & Hi'); try eassumption.
+            reflexivity. now firstorder. symmetry.
+            reflexivity. now firstorder.
+            destruct (lt_dec (c1 - 1) 1).
+            + eexists. eexists id. repeat split. unfold AppClo.
+              eapply Eval_proj_per_cc; eauto.
+              simpl. omega. reflexivity.
+              now econstructor; simpl; eauto.
+              eapply injective_subdomain_Empty_set.
+              rewrite <- !plus_n_O.
+              eapply Hbase; try eassumption.
+              rewrite cc_approx_val_eq. now eauto.
+            + eexists. eexists id. repeat split. unfold AppClo.
+              eapply Eval_proj_per_cc; eauto.
+              simpl. omega. reflexivity.
+              eapply Eval_proj_per_cc; eauto.
+              simpl. omega.
+              rewrite M.gso. eassumption.
+              intros Heq; subst. now eauto with Ensembles_DB.
+              reflexivity. 
+              econstructor; try (now simpl; eauto). simpl.
+              erewrite <- Forall2_length; [| eassumption ]. simpl in *. omega.
+              now eapply injective_subdomain_Empty_set.
+              rewrite <- plus_n_O.
+              eapply Hbase; try eassumption.
+              now rewrite cc_approx_val_eq. }
+      (* Termination *) 
+      - { simpl in Hcost.
+          eapply Forall2_monotonic_strong in Hall; (* yiiiiiikes *)
+            [| intros x1 x2 Hin1 Hin2 Hyp;
+               eapply (cc_approx_var_env_heap_env_equiv
+                         _ _
+                         (occurs_free (Eapp f1 t xs1))
+                         (occurs_free (AppClo clo_tag f2 t xs2 f2' Γ))) in Hyp;
+               [ now eapply Hyp | eassumption | eassumption | eassumption | eassumption
+                 | normalize_occurs_free; now eauto with Ensembles_DB
+                 | unfold AppClo; repeat normalize_occurs_free; rewrite FromList_cons ];
+               right; constructor;
+               [ right; constructor;
+               [ now eauto with Ensembles_DB
+               | now intros Hc; inv Hc; eapply Hnin1; eauto ]
+               | now intros Hc; inv Hc; eapply Hnin2; eauto ] ].
+          edestruct (cc_approx_var_env_getlist IIG IG  k j rho1' rho2') as [vs2 [Hgetl' Hcc']];
+            [ eassumption | now eauto |].
+          edestruct Hvar as [l2 [Hget' Hcc]]; eauto.
+          simpl in Hcc. rewrite Hgetl in Hcc. destruct l2 as [l2 | ]; [| contradiction ]. 
+          destruct (get l2 H2') as [v |] eqn:Hget2; try contradiction.
+          destruct Hcc as [Hbeq Hcc]. simpl in Hcc.
+          destruct v as [ ? [| [| B2 f3 ] [| [ env_loc' |] [|] ]] | | ]; try contradiction.
+          edestruct Hcc as (Him & xs2' & e2 & rho2'' & Hfind' & Hset' & Hi'); try eassumption.
+          reflexivity. now firstorder. reflexivity. now firstorder.
+          edestruct (live_exists' (env_locs rho2'' (occurs_free e2)) H2') as [H2'' Hgc'].
+          assert (Hgc1 := Hgc); assert (Hgc2 := Hgc').
+          destruct Hgc as [Hseq [bgc [Heqgc Hinjgc]]].
+          destruct Hgc' as [Hseq' [bgc' [Heqgc' Hinjgc']]].
+          edestruct Hi' with (i := k - cost  (Eapp f1 t xs1))
+                               (j' := j) as [HG [r2 [c2 [m2 [b2' [Hbs2 [Hinj [HIG Hcc2]]]]]]]];
+            [ | omega | | | | | | | | | eassumption | | ].  
+          + simpl. omega.
+          + rewrite compose_id_neut_r. rewrite compose_id_neut_l. reflexivity.
+          + eapply Forall2_monotonic_strong; [| eassumption ].
+            intros v v' Hinv1 Hinv2 Heq. rewrite cc_approx_val_eq.
+            eapply cc_approx_val_monotonic with (k := k).
+            assert (Hrv : val_loc v \subset env_locs rho1' (occurs_free (Eapp f1 t xs1))).
+            { normalize_occurs_free. rewrite env_locs_Union.
+              eapply Included_Union_preserv_l. rewrite env_locs_FromList.
+              simpl. eapply In_Union_list.
+              eapply in_map. eassumption. eassumption. }
+            assert (Hrv' : val_loc v' \subset
+                                   env_locs rho2' (occurs_free (AppClo clo_tag f2 t xs2 f2' Γ))).
+            { unfold AppClo. repeat normalize_occurs_free.
+              rewrite FromList_cons, !Setminus_Union_distr, !env_locs_Union.
+              do 2 eapply Included_Union_preserv_r.
+              eapply Included_Union_preserv_l. eapply Included_Union_preserv_r.
+              rewrite !Setminus_Disjoint.
+              rewrite env_locs_FromList.
+              simpl. eapply In_Union_list.
+              eapply in_map. eassumption. eassumption. 
+              now eapply Disjoint_Singleton_r; intros Hc; eapply Hnin1; eauto.
+              now eapply Disjoint_Singleton_r; intros Hc; inv Hc; eapply Hnin2; eauto. }
+            eapply cc_approx_val_heap_monotonic;
+              [ | | | | | now eapply HL.subheap_refl | ].
+            * eapply well_formed_respects_heap_env_equiv in Hwf1; [| eassumption ].
+              eapply well_formed_antimon; [| now apply Hwf1 ].
+              now eapply reach'_set_monotonic.
+            * eapply well_formed_respects_heap_env_equiv in Hwf2; [| eassumption ].
+              eapply well_formed_antimon; [| now apply Hwf2 ].
+              now eapply reach'_set_monotonic.
+            * eapply Included_trans; [| eapply reachable_in_dom; try eassumption ].
+              eapply Included_trans; [| now eapply reach'_extensive ].
+              eassumption.
+              eapply well_formed_respects_heap_env_equiv in Hwf1; [| eassumption ].
+              eassumption.
+              eapply env_locs_in_dom; eassumption.
+            * eapply Included_trans; [| eapply reachable_in_dom; try eassumption ].
+              eapply Included_trans; [| now eapply reach'_extensive ].
+              eassumption.
+              eapply well_formed_respects_heap_env_equiv in Hwf2; [| eassumption ].
+              eassumption.
+              eapply env_locs_in_dom; eassumption.
+            * eapply def_funs_subheap. eauto.
+            * eassumption.
+            * simpl; omega.
+          + eapply heap_env_equiv_heap_equiv. eassumption.
+          + eassumption.
+          + eapply heap_env_equiv_heap_equiv. eassumption.
+          + eassumption.
+          + eapply IInvGC; try eassumption.
+          + simpl; omega.
+          + intros i.
+            edestruct (Hstuck1 (i + cost (Eapp f1 t xs1))) as [r' [m' Hstep']].
+            inv Hstep'.
+            * omega.
+            * rewrite NPeano.Nat.add_sub in Hbs0.
+              repeat subst_exp. 
+              edestruct live_deterministic as [b1' [b2' [Heq [Hinj1' Hinj2']]]].
+              now apply Hgc1. now apply Hgc. try eassumption.
+              edestruct big_step_gc_heap_env_equiv_r
+                as [r1 [m1 [b1'' [b2''[Hgc'' _]]]]].
+              eassumption.
+              eapply heap_env_equiv_heap_equiv. symmetry. eassumption.
+              eassumption. eassumption. do 2 eexists. eassumption.
+          + do 3 eexists. exists b2'. repeat split.
+            * eapply Eval_proj_per_cc with
+              (c := c2 + 1 + 1 + cost (Eapp f2' t (Γ :: xs2))).
+              simpl; omega.
+              eassumption. eassumption. reflexivity.
+              eapply Eval_proj_per_cc. simpl; omega.
+              rewrite M.gso. eassumption.
+              intros Hc. subst. eapply Hnin2. now left; eauto.
+              eassumption. reflexivity. simpl.
+              eapply Eval_app_per_cc.
+              simpl. omega.
+              rewrite M.gso. rewrite M.gss. reflexivity.
+              now intros Hc; subst; eauto.
+              eassumption.
+              simpl. rewrite M.gss.
+              rewrite !getlist_set_neq. now rewrite Hgetl'.
+              intros Hc. eapply Hnin2. now eauto.
+              intros Hc. eapply Hnin1. now eauto.
+              now eauto. eassumption. reflexivity. simpl.
+              replace (c2 + 1 + 1 + S (S (length xs2)) - 1 - 1 - S (S (length xs2)))  with c2.
+              eassumption. omega.
+            * eassumption.
+            * admit.
+              (* eapply Hinv; try eassumption. *)
+              (* eapply InvGC in HIG; try eassumption. *)
+              (* replace c1 with ((c1 - cost (Eapp f1 t xs1)) + cost (Eapp f1 t xs1)) *)
+              (*   by (simpl in *; omega). *)
+              (* eapply LInvHeapEquiv.  *)
+              (* eassumption. *)
+              (* eapply Hinv. Hinv. *)
+              (* eapply LInvGC; try eassumption. *)
+              (* eapply Hinv. IInvAppCompat; try eassumption. *)
+            * rewrite cc_approx_val_eq in *. eapply cc_approx_val_monotonic.
+              eassumption. simpl. omega. }        
+    Admitted.
+    
+    
+    (** * Heap allocation and environment extension properties *)
+
+    
 
       
     (** Constructor compatibility *)
     Lemma cc_approx_exp_constr_compat (k j : nat)
           (b : Inj) (H1 H2 : heap block)  (rho1 rho2 : env)
-          (x1 x2 : var) (t : cTag) (ys1 ys2 : list var) (e1 e2 : exp) (r1 r2 : nat)
-          
-          (IInvConstrCompat :
-             forall (H1 H2 H1' H2' : heap block) (rho1 rho2 : env)
-               (b1 b2 : block) (l1 l2 : loc),
-               IIL1 (H1, rho1, Econstr x1 t ys1 e1) (H2, rho2, Econstr x2 t ys2 e2) ->
-               alloc b1 H1 = (l1, H1') -> 
-               alloc b2 H2 = (l2, H2') ->
-               size_val b1 = size_val b2 ->
-               locs b1 \subset reach' H1 (env_locs rho1 (occurs_free (Econstr x1 t ys1 e1))) ->
-               locs b2 \subset reach' H2 (env_locs rho2 (occurs_free (Econstr x2 t ys2 e2))) ->
-               IIL2 (H1', M.set x1 (Loc l1) rho1, e1) (H2', M.set x2 (Loc l2) rho2, e2)) : 
-
+          (x1 x2 : var) (t : cTag) (ys1 ys2 : list var) (e1 e2 : exp)  : 
+      InvCtxCompat IL1 IL2 H1 H2 rho1 rho2 (Econstr_c x1 t ys1 Hole_c) (Econstr_c x2 t ys2 Hole_c) e1 e2 ->
+      IInvCtxCompat IIL1 IIL2 H1 H2 rho1 rho2 (Econstr_c x1 t ys1 Hole_c) (Econstr_c x2 t ys2 Hole_c) e1 e2 ->
+      InvCostBase IL1 IIL1 H1 H2 rho1 rho2 (Econstr x1 t ys1 e1) (Econstr x2 t ys2 e2)  ->
+      
       well_formed (reach' H1 (env_locs rho1 (occurs_free (Econstr x1 t ys1 e1)))) H1 ->
       well_formed (reach' H2 (env_locs rho2 (occurs_free (Econstr x2 t ys2 e2)))) H2 ->
       (env_locs rho1 (occurs_free (Econstr x1 t ys1 e1))) \subset dom H1 ->
@@ -88,10 +558,8 @@ Module Compat (H : Heap).
 
       (forall j, Forall2 (cc_approx_var_env k j IIG IG b H1 rho1 H2 rho2) ys1 ys2) ->
 
-      (r1 - r2) <= F*(cost H1 rho1 (Econstr x1 t ys1 e1)) ->
-
       (forall vs1 vs2 l1 l2 H1' H2',
-         k >= cost H1 rho1 (Econstr x1 t ys1 e1) ->
+         k >= cost (Econstr x1 t ys1 e1) ->
          (* allocate a new location for the constructed value *)
          alloc (Constr t vs1) H1 = (l1, H1') ->
          alloc (Constr t vs2) H2 = (l2, H2') ->
@@ -99,22 +567,22 @@ Module Compat (H : Heap).
          locs (Constr t vs1) \subset env_locs rho1 (occurs_free (Econstr x1 t ys1 e1)) ->
          locs (Constr t vs2) \subset env_locs rho2 (occurs_free (Econstr x2 t ys2 e2)) ->
          (* and related *)
-         (forall j, Forall2 (fun l1 l2 => (Res (l1, H1)) ≺ ^ (k - cost H1 rho1 (Econstr x1 t ys1 e1) ; j ; IIG ; IG ; b) (Res (l2, H2))) vs1 vs2) ->
-         (forall j, (e1, M.set x1 (Loc l1) rho1, H1') ⪯ ^ (k - cost H1 rho1 (Econstr x1 t ys1 e1) ; j ; IIL2 ; IIG ; ILi r2 ; IG)
+         (forall j, Forall2 (fun l1 l2 => (Res (l1, H1)) ≺ ^ (k - cost (Econstr x1 t ys1 e1) ; j ; IIG ; IG ; b) (Res (l2, H2))) vs1 vs2) ->
+         (forall j, (e1, M.set x1 (Loc l1) rho1, H1') ⪯ ^ (k - cost (Econstr x1 t ys1 e1) ; j ; IIL2 ; IIG ; IL2 ; IG)
                (e2, M.set x2 (Loc l2) rho2, H2'))) ->
       
-      (Econstr x1 t ys1 e1, rho1, H1) ⪯ ^ (k ; j ; IIL1 ; IIG ; ILi r1 ; IG) (Econstr x2 t ys2 e2, rho2, H2).
+      (Econstr x1 t ys1 e1, rho1, H1) ⪯ ^ (k ; j ; IIL1; IIG ; IL1 ; IG) (Econstr x2 t ys2 e2, rho2, H2).
     Proof with now eauto with Ensembles_DB.
-      intros Hwf1 Hwf2 Hdom1 Hdom2 Hall Hleq Hpre b1 b2 H1' H2' rho1' rho2' v1 c1 m1
+      intros Hinv Hiinv Hbase Hwf1 Hwf2 Hdom1 Hdom2 Hall Hpre b1 b2 H1' H2' rho1' rho2' v1 c1 m1
              Heq1 Hinj1 Heq2 Hinj2 HII Hleq1 Hstep1 Hstuck1.
       assert (Hall' := Hall).
       inv Hstep1.
       (* Timeout! *)
-      - { exists OOT, (c1 - r1). eexists. exists  id. repeat split. 
+      - { exists OOT, c1. eexists. exists id. repeat split. 
           - econstructor. simpl. specialize (Hall 0). erewrite <- Forall2_length; [| eassumption ].
             simpl in Hcost. omega. reflexivity.
           - simpl. eapply injective_subdomain_Empty_set. 
-          - eapply InvCostTimeout. eassumption.
+          - eapply Hbase; try eassumption.
           - now rewrite cc_approx_val_eq. }
       (* Termination *)
       - { edestruct (cc_approx_var_env_getlist IIG IG k j rho1' rho2') as [vs2 [Hget' Hpre']];
@@ -303,69 +771,60 @@ Module Compat (H : Heap).
             eapply Included_Union_preserv_l. 
             rewrite env_locs_FromList; eauto. reflexivity.
               
-          - eapply IInvConstrCompat; [ eassumption | eassumption | eassumption | | | ].
-            simpl.
-            eapply getlist_length_eq in Hget.
-            eapply getlist_length_eq in Hget'. congruence.
-            eapply Included_trans; [| now eapply reach'_extensive ].
-            normalize_occurs_free. rewrite env_locs_Union.
-            eapply Included_Union_preserv_l. rewrite env_locs_FromList.
-            simpl. reflexivity. eassumption.
-            eapply Included_trans; [| now eapply reach'_extensive ].
-            normalize_occurs_free. rewrite env_locs_Union.
-            eapply Included_Union_preserv_l. rewrite env_locs_FromList.
-            simpl. reflexivity. eassumption.
+          - eapply Hiinv; try eassumption.
+            econstructor; eauto.
+            now econstructor; eauto.
+            econstructor; eauto.
+            now econstructor; eauto.
           - simpl. simpl in Hcost. omega.
-          - intros i. edestruct (Hstuck1 (i + cost H1' rho1' (Econstr x1 t ys1 e1))) as [r' [m' Hstep']].
+          - intros i. edestruct (Hstuck1 (i + cost (Econstr x1 t ys1 e1))) as [r' [m' Hstep']].
             inv Hstep'.
             * omega.
             * rewrite NPeano.Nat.add_sub in Hbs0. repeat subst_exp.
               repeat eexists; eauto.  
           - repeat eexists; eauto.
-            + eapply Eval_constr_per_cc with (c := c2 + cost H1' rho1' (Econstr x2 t ys2 e2))
+            + eapply Eval_constr_per_cc with (c := c2 + cost (Econstr x2 t ys2 e2))
               ; [ | | | rewrite NPeano.Nat.add_sub ]; try eassumption.
-              simpl. omega.
-            + simpl. eapply InvCompat_str with (c2' := S (length ys1)).
-              replace (length ys2) with (length ys1).
-              replace (c2 + S (length ys1) - S (length ys1)) with c2 by omega.
-              eassumption. simpl. simpl in Hleq. omega.
+              simpl. omega. 
+            + eapply Hinv with (c2':= cost (Econstr x2 t ys2 e2)); try eassumption.
+              replace (c2 + cost (Econstr x2 t ys2 e2) - cost (Econstr x2 t ys2 e2)) with c2 by omega. 
+              eassumption.
+              replace (cost (Econstr x1 t ys1 e1)) with (0 + cost_ctx (Econstr_c x1 t ys1 Hole_c)) by (simpl; omega).
+              econstructor; eauto. now econstructor; eauto.
+              replace (cost (Econstr x2 t ys2 e2)) with (0 + cost_ctx (Econstr_c x2 t ys2  Hole_c)) by (simpl; omega).
+              econstructor; eauto. now econstructor; eauto.
             + rewrite cc_approx_val_eq. eapply cc_approx_val_monotonic.
               rewrite <- cc_approx_val_eq. eassumption. simpl in *. omega. }
     Qed.
     
     (** Projection compatibility *)
     Lemma cc_approx_exp_proj_compat (k : nat) (H1 H2 : heap block) (rho1 rho2 : env) (b : Inj)
-          (x1 x2 : var) (t : cTag) (n : N) (y1 y2 : var) (e1 e2 : exp) (r1 r2 : nat)
+          (x1 x2 : var) (t : cTag) (n : N) (y1 y2 : var) (e1 e2 : exp) :
 
-          (IInvProjCompat :
-             forall (H1 H2 : heap block) (rho1 rho2 : env) (v1 v2 : value),
-               IIL1 (H1, rho1, Eproj x1 t n y1 e1) (H2, rho2, Eproj x2 t n y2 e2) ->
-               val_loc v1 \subset reach' H1 (env_locs rho1 (occurs_free (Eproj x1 t n y1 e1))) ->
-               val_loc v2 \subset reach' H2 (env_locs rho2 (occurs_free (Eproj x2 t n y2 e2))) ->
-               IIL2 (H1, M.set x1 v1 rho1, e1) (H2, M.set x2 v2 rho2, e2)) :
-
+      InvCtxCompat IL1 IL2 H1 H2 rho1 rho2 (Eproj_c x1 t n y1 Hole_c) (Eproj_c x2 t n y2 Hole_c) e1 e2 ->
+      IInvCtxCompat IIL1 IIL2 H1 H2 rho1 rho2 (Eproj_c x1 t n y1 Hole_c) (Eproj_c x2 t n y2 Hole_c) e1 e2 ->
+      InvCostBase IL1 IIL1 H1 H2 rho1 rho2 (Eproj x1 t n y1 e1) (Eproj x2 t n y2 e2) ->
+      
       (forall j, cc_approx_var_env k j IIG IG b H1 rho1 H2 rho2 y1 y2) ->
 
-      r1 - r2 <= F*(cost H1 rho1 (Eproj x1 t n y1 e1)) ->
-
-      (forall v1 v2,
-         k >= cost H1 rho1 (Eproj x1 t n y1 e1) ->
-         (forall j, (Res (v1, H1)) ≺ ^ (k - cost H1 rho1 (Eproj x1 t n y1 e1) ; j ; IIG ; IG; b) (Res (v2, H2))) ->
-         (forall j, (e1, M.set x1 v1 rho1, H1) ⪯ ^ (k - cost H1 rho1 (Eproj x1 t n y1 e1) ; j ; IIL2 ; IIG ; ILi r2 ; IG) (e2, M.set x2 v2 rho2, H2))) ->
       
-      (forall j, (Eproj x1 t n y1 e1, rho1, H1) ⪯ ^ (k ; j ; IIL1 ; IIG ; ILi r1 ; IG) (Eproj x2 t n y2 e2, rho2, H2)).
+      (forall v1 v2,
+         (forall j, (Res (v1, H1)) ≺ ^ (k - cost (Eproj x1 t n y1 e1) ; j ; IIG ; IG; b) (Res (v2, H2))) ->
+         (forall j, (e1, M.set x1 v1 rho1, H1) ⪯ ^ (k - cost (Eproj x1 t n y1 e1) ; j ; IIL2 ; IIG ; IL2 ; IG) (e2, M.set x2 v2 rho2, H2))) ->
+      
+      (forall j, (Eproj x1 t n y1 e1, rho1, H1) ⪯ ^ (k ; j ; IIL1 ; IIG ; IL1 ; IG) (Eproj x2 t n y2 e2, rho2, H2)).
     Proof with (now eauto with Ensembles_DB).
-      intros Hall Hleq Hpre j b1 b2 H1' H2' rho1' rho2' v1 c1 m1
+      intros Hinv Hiinv Hbase Hall Hpre j b1 b2 H1' H2' rho1' rho2' v1 c1 m1
              Heq1' Hinj1 Heq2' Hinj2 HII Hleq1 Hstep1 Hstuck. inv Hstep1.
       (* Timeout! *)
-      - { simpl in Hcost. exists OOT, (c1 - r1). eexists. exists id. repeat split. 
+      - { simpl in Hcost. exists OOT, c1. eexists. exists id. repeat split. 
           - econstructor. simpl; omega. reflexivity.
           - eapply injective_subdomain_Empty_set.
-          - eapply InvCostTimeout. eassumption.
+          - eapply Hbase; eauto.
           - now rewrite cc_approx_val_eq. }
       (* Termination *)
-      - { pose (cost1 := cost H1' rho1' (Eproj x1 t n y1 e1)).
-          pose (cost2 := cost H2' rho2' (Eproj x2 t n y2 e2)).
+      - { pose (cost1 := cost (Eproj x1 t n y1 e1)).
+          pose (cost2 := cost (Eproj x2 t n y2 e2)).
           assert (Hall' := Hall).
           
           eapply (cc_approx_var_env_heap_env_equiv
@@ -412,8 +871,7 @@ Module Compat (H : Heap).
           eapply Forall2_symm_strong; [| eassumption ]. intros. now symmetry; eauto. eassumption.
           
           edestruct Hpre with (c1 := c1 - cost1) as [v2 [c2 [m2 [b' [Hstep [Hinj' [HS Hres]]]]]]];
-            [ | | | | | | | | eassumption | | ].  
-          - simpl in *; omega. 
+            [ | | | | | | | eassumption | | ].  
           - intros j'.
             
             edestruct (Hall' (S j'))  as [l2'' [Hgetl2'' Hcc'']]; eauto. repeat subst_exp. 
@@ -466,15 +924,11 @@ Module Compat (H : Heap).
 
             eapply Included_trans; [| eapply reach'_extensive ].
             eapply env_locs_monotonic. normalize_occurs_free...
-          - eapply IInvProjCompat. eassumption.
-            eapply Included_trans; [| eapply Included_post_reach' ].
-            normalize_occurs_free. rewrite env_locs_Union, post_Union. eapply Included_Union_preserv_l.
-            rewrite env_locs_Singleton; eauto. simpl. erewrite post_Singleton; eauto.
-            simpl. eapply In_Union_list. eapply in_map. eapply nthN_In. eassumption.
-            eapply Included_trans; [| eapply Included_post_reach' ].
-            normalize_occurs_free. rewrite env_locs_Union, post_Union. eapply Included_Union_preserv_l.
-            rewrite env_locs_Singleton; eauto. simpl. erewrite post_Singleton; eauto.
-            simpl. eapply In_Union_list. eapply in_map. eapply nthN_In. eassumption.
+          - eapply Hiinv; try eassumption.
+            econstructor; eauto.
+            now econstructor; eauto.
+            econstructor; eauto.
+            now econstructor; eauto.
           - unfold cost1. simpl. omega. 
           - intros i. edestruct (Hstuck (i + cost1)) as [r' [m' Hstep']].
             inv Hstep'.
@@ -485,67 +939,61 @@ Module Compat (H : Heap).
           - repeat eexists; eauto. eapply Eval_proj_per_cc with (c := c2 + cost2); try eassumption.
             unfold cost2. simpl; omega. simpl. rewrite NPeano.Nat.add_sub.
             eassumption.
-            eapply InvCompat_str with (c2' := cost1).
-            unfold cost1, cost2. simpl. rewrite NPeano.Nat.add_sub. eassumption. 
-            simpl; simpl in Hleq; omega.
+            eapply Hinv with (c2':= cost2); try eassumption.
+            replace (c2 + cost2 - cost2) with c2 by omega. 
+            eassumption.
+            replace cost1 with (0 + cost_ctx (Eproj_c x1 t n y1 Hole_c)) by (unfold cost1; simpl; omega).
+            econstructor; eauto. now econstructor; eauto.
+            replace cost2 with (0 + cost_ctx (Eproj_c x2 t n y2 Hole_c)) by (unfold cost2; simpl; omega).
+            econstructor; eauto. now econstructor; eauto.
             rewrite cc_approx_val_eq in *.
             eapply cc_approx_val_monotonic. eassumption.
             unfold cost1, cost2. simpl. simpl in Hcost. omega. }
     Qed.
     
     (** Case compatibility *)
-    Lemma cc_approx_exp_case_nil_compat (k j : nat) (H1 H2 : heap block) (rho1 rho2 : env) (x1 x2 : var) (c : nat) :
-      c <= F * (cost H1 rho1 (Ecase x1 [])) -> 
-      (Ecase x1 [], rho1, H1) ⪯ ^ (k ; j ; IIL1 ; IIG ; ILi c ; IG) (Ecase x2 [], rho2, H2).
+    Lemma cc_approx_exp_case_nil_compat (k j : nat) (H1 H2 : heap block) (rho1 rho2 : env) (x1 x2 : var) :
+      InvCostBase IL1 IIL1 H1 H2 rho1 rho2 (Ecase x1 []) (Ecase x2 []) ->
+      (Ecase x1 [], rho1, H1) ⪯ ^ (k ; j ; IIL1; IIG ; IL1 ; IG) (Ecase x2 [], rho2, H2).
     Proof.
-      intros Hleq b1 b2 H1' H2' rho1' rho2' v1 c1 m1 Heq1 Hinj1 Heq2 Hinj2 HII Hleq1 Hstep1 Hns. inv Hstep1.
+      intros Hbase b1 b2 H1' H2' rho1' rho2' v1 c1 m1 Heq1 Hinj1 Heq2 Hinj2 HII Hleq1 Hstep1 Hns. inv Hstep1.
       (* Timeout! *)
-      - { simpl in Hcost. exists OOT, (c1 - c). eexists. eexists id. repeat split. 
+      - { simpl in Hcost. exists OOT, c1. eexists. eexists id. repeat split. 
           - econstructor. simpl; omega. reflexivity. 
           - now firstorder.
-          - eapply InvCostTimeout.
-            eassumption.
+          - eapply Hbase; eassumption.
           - now rewrite cc_approx_val_eq. }
-      (* Termination *)
+      (* Termination *) 
       - { simpl in Htag. discriminate. }
     Qed.
     
     Lemma cc_approx_exp_case_compat (k j : nat) (b : Inj) (H1 H2 : heap block) (rho1 rho2 : env) (x1 x2 : var) (t : cTag)
-          (e1 e2 : exp) (Pats1 Pats2 : list (cTag * exp)) (r1 r2 : nat)
- 
-      (IInvCaseHdCompat :
-         forall (H1 H2 : heap block) (rho1 rho2 : env),
-           IIL1 (H1, rho1, Ecase x1 ((t, e1) :: Pats1)) (H2, rho2, Ecase x2 ((t, e2) :: Pats2)) ->
-           IIL2 (H1, rho1, e1) (H2, rho2, e2))
-
-      (IInvCaseTlCompat :
-         forall (H1 H2 : heap block) (rho1 rho2 : env),
-           IIL1 (H1, rho1, Ecase x1 ((t, e1) :: Pats1)) (H2, rho2, Ecase x2 ((t, e2) :: Pats2)) ->
-           IIL1 (H1, rho1, Ecase x1 Pats1) (H2, rho2, Ecase x2 Pats2)) :
-        
+          (e1 e2 : exp) (Pats1 Pats2 : list (cTag * exp)) :
+      InvCostBase IL1 IIL1 H1 H2 rho1 rho2 (Ecase x1 ((t, e1) :: Pats1)) (Ecase x2 ((t, e2) :: Pats2)) -> 
+      IInvCaseHdCompat IIL1 IIL2 H1 H2 rho1 rho2 x1 x2 t Pats1 Pats2 e1 e2 ->
+      InvCaseHdCompat IL1 IL2 H1 H2 rho1 rho2 x1 x2 t Pats1 Pats2 e1 e2 ->
+      IInvCaseTlCompat IIL1 H1 H2 rho1 rho2 x1 x2 t Pats1 Pats2 e1 e2 -> 
+      InvCaseTlCompat IL1 H1 H2 rho1 rho2 x1 x2 t Pats1 Pats2 e1 e2  ->
+      
       cc_approx_var_env k j IIG IG b H1 rho1 H2 rho2 x1 x2 ->
 
-      (r1 - r2) <= F * (cost H1 rho1 (Ecase x1 Pats1)) -> 
+      (e1, rho1, H1) ⪯ ^ (k - cost (Ecase x1 Pats1); j; IIL2 ; IIG ; IL2 ; IG) (e2, rho2, H2) ->
 
-      (forall H1 H2 rho1 rho2,
-         k >= cost H1 rho1 (Ecase x1 Pats1) ->
-         (e1, rho1, H1) ⪯ ^ (k - cost H1 rho1 (Ecase x1 Pats1); j; IIL2 ; IIG ; ILi r2 ; IG) (e2, rho2, H2)) ->
+      (Ecase x1 Pats1, rho1, H1) ⪯ ^ (k ; j ; IIL1 ; IIG ; IL1 ; IG) (Ecase x2 Pats2, rho2, H2) ->
 
-      (Ecase x1 Pats1, rho1, H1) ⪯ ^ (k ; j ; IIL1 ; IIG ; ILi r1 ; IG) (Ecase x2 Pats2, rho2, H2) ->
-
-      (Ecase x1 ((t, e1) :: Pats1), rho1, H1) ⪯ ^ (k ; j ; IIL1 ; IIG ; ILi r1 ; IG) (Ecase x2 ((t, e2) :: Pats2), rho2, H2).
+      (Ecase x1 ((t, e1) :: Pats1), rho1, H1) ⪯ ^ (k ; j ; IIL1 ; IIG ; IL1 ; IG) (Ecase x2 ((t, e2) :: Pats2), rho2, H2).
     Proof with now eauto with Ensembles_DB.
-      intros Hvar Hleq Hexp_hd Hexp_tl b1 b2 H1' H2' rho1' rho2'
+      intros Hbase Hiinvh Hinvh Hiinvt Hinvt Hvar Hexp_hd Hexp_tl b1 b2 H1' H2' rho1' rho2'
              v1 c1 m1 Heq1 Hinj1 Heq2 Hinj2 HII Hleq1 Hstep1 Hstuck1.
       inv Hstep1.
       (* Timeout! *)
-      - { simpl in Hcost. exists OOT, (c1 - r1). eexists. exists id. repeat split. 
+      - { simpl in Hcost. exists OOT, c1. eexists. exists id. repeat split. 
           - econstructor. simpl; omega. reflexivity. 
           - eapply injective_subdomain_Empty_set.
-          - eapply InvCostTimeout. eassumption.
+          - eapply Hbase; eassumption.
           - now rewrite cc_approx_val_eq. }
-      - { pose (cost1 := cost H1' rho1' (Ecase x1 ((t, e1) :: Pats1))).
-          pose (cost2 := cost H2' rho2' (Ecase x2 ((t, e2) :: Pats2))).
+      - { pose (cost1 := cost (Ecase x1 ((t, e1) :: Pats1))).
+          pose (cost2 := cost (Ecase x2 ((t, e2) :: Pats2))).
           eapply (cc_approx_var_env_heap_env_equiv
                     _ _
                     (occurs_free (Ecase x1 ((t, e1) :: Pats1)))
@@ -560,8 +1008,7 @@ Module Compat (H : Heap).
           destruct Hcc as [Heq Hall']; subst. simpl in Hall', Hcost.
           simpl in Htag. destruct (M.elt_eq t t') eqn:Heq; subst.
           - inv Htag.
-            edestruct Hexp_hd with (c1 := c1 - cost1) as [v2 [c2 [m2 [b' [Hstep [Hinj' [HS Hres]]]]]]]. 
-            + simpl in *; omega.
+            edestruct Hexp_hd with (c1 := c1 - cost1) as [v2 [c2 [m2 [b' [Hstep [Hinj' [HS Hres]]]]]]].
             + eapply heap_env_equiv_antimon. now eapply Heq1.
               normalize_occurs_free...
             + eapply injective_subdomain_antimon. eassumption.
@@ -572,7 +1019,7 @@ Module Compat (H : Heap).
             + eapply injective_subdomain_antimon. eassumption.
               eapply reach'_set_monotonic. eapply env_locs_monotonic.
               normalize_occurs_free...
-            + eapply IInvCaseHdCompat; eassumption.
+            + eapply Hiinvh; try eassumption.
             + unfold cost1. simpl; omega.
             + eassumption.
             + intros i. edestruct (Hstuck1 (i + cost1)) as [r' [m'' Hstep']].
@@ -587,9 +1034,9 @@ Module Compat (H : Heap).
               * eapply Eval_case_per_cc with (c := c2 + cost2)
                 ; [ | | | | rewrite NPeano.Nat.add_sub ]; try eassumption.
                 unfold cost2. omega. now simpl; rewrite Heq. 
-              * simpl. eapply InvCompat_str with (c2' := cost1).
-                unfold cost2, cost1. simpl. rewrite NPeano.Nat.add_sub.
-                eassumption. simpl; simpl in Hleq; omega.
+              * eapply Hinvh; try eassumption.
+                replace (c2 + cost2 - cost (Ecase x2 ((t', e2) :: Pats2))) with c2 by (unfold cost2; omega).
+                eassumption.
               * rewrite cc_approx_val_eq. eapply cc_approx_val_monotonic.
                 rewrite <- cc_approx_val_eq. eassumption. unfold cost1. simpl. omega.
           - edestruct Hexp_tl as [v2 [c2 [m2 [b' [Hstep2 [Hinj' [HS Hpre2]]]]]]];
@@ -604,7 +1051,7 @@ Module Compat (H : Heap).
             + eapply injective_subdomain_antimon. eassumption.
               eapply reach'_set_monotonic. eapply env_locs_monotonic.
               normalize_occurs_free...
-            + eapply IInvCaseTlCompat; eassumption.
+            + eapply Hiinvt; try eassumption. 
             + simpl in Hcost. omega.
             + intros i. edestruct (Hstuck1 i) as [r' [m'' Hstep']].
               inv Hstep'.
@@ -620,7 +1067,8 @@ Module Compat (H : Heap).
                 { simpl in Hcost0. exists OOT, c2. eexists. exists b'. repeat split.
                   - econstructor. simpl. eassumption. reflexivity. 
                   - eassumption.
-                  - eassumption.
+                  - eapply Hinvt; try eassumption.
+                    
                   - eassumption. }
               * (* termination *)
                 { repeat eexists; eauto.
@@ -631,27 +1079,26 @@ Module Compat (H : Heap).
     Qed.
     
     (** Halt compatibility *)
-    Lemma cc_approx_exp_halt_compat (k j : nat) (H1 H2 : heap block) (rho1 rho2 : env) (b : Inj) (x1 x2 : var) (r : nat) :
-      r <= F * (cost H1 rho1 (Ehalt x1)) -> 
-          
+    Lemma cc_approx_exp_halt_compat (k j : nat) (H1 H2 : heap block) (rho1 rho2 : env) (b : Inj) (x1 x2 : var) :
+      InvCostBase IL1 IIL1 H1 H2 rho1 rho2 (Ehalt x1) (Ehalt x2) ->
+      
       cc_approx_var_env k j IIG IG b H1 rho1 H2 rho2 x1 x2 ->
       injective_subdomain (reach_n H1 j (env_locs rho1 [set x1])) b ->
-
-      (Ehalt x1, rho1, H1) ⪯ ^ (k ; j ; IIL1 ; IIG ; ILi r ; IG) (Ehalt x2, rho2, H2).
+      
+      (Ehalt x1, rho1, H1) ⪯ ^ (k ; j ; IIL1 ; IIG ; IL1; IG) (Ehalt x2, rho2, H2).
     Proof.
-      intros Hleq Hvar Hinj b1 b2 H1' H2' rho1' rho2' v1 c1 m1 Heq1 Hinj1
+      intros Hbase Hvar Hinj b1 b2 H1' H2' rho1' rho2' v1 c1 m1 Heq1 Hinj1
              Heq2 Hinj2 Hleq1 HII Hstep1 Hstuck1.
       assert (Hvar' := Hvar).
       inv Hstep1.
       - (* Timeout! *)
-        { simpl in Hcost. exists OOT, (c1 - r). eexists. exists id. repeat split. 
-          - econstructor; eauto. simpl. omega.
+        { simpl in Hcost. exists OOT, c1. eexists. exists id. repeat split. 
+          - econstructor; eauto.
           - eapply injective_subdomain_Empty_set.
-          - rewrite <- plus_n_O. eapply InvCostTimeout.
-            eassumption.
+          - rewrite <- plus_n_O. eapply Hbase; try eassumption.
           - now rewrite cc_approx_val_eq. }
-      - pose (cost1 := cost H1' rho1' (Ehalt x1)).
-        pose (cost2 := cost H2' rho2' (Ehalt x2)).
+      - pose (cost1 := cost (Ehalt x1)).
+        pose (cost2 := cost (Ehalt x2)).
         eapply (cc_approx_var_env_heap_env_equiv
                   _ _
                   (occurs_free (Ehalt x1))
@@ -686,7 +1133,7 @@ Module Compat (H : Heap).
           rewrite Hvar'.
           eapply injective_subdomain_antimon. eassumption.
           simpl. rewrite occurs_free_Ehalt. eapply reach_n_in_reach.
-        * eapply InvCostBase. eassumption. eassumption.
+        * eapply Hbase; try eassumption.
         * rewrite cc_approx_val_eq in *.
           eapply cc_approx_val_monotonic. eassumption.
           omega.
@@ -718,45 +1165,37 @@ Module Compat (H : Heap).
       - simpl. rewrite Setminus_Empty_set_neut_r. reflexivity.
     Qed.
 
-
+   
     (** Abstraction compatibility *)
-    Lemma cc_approx_exp_fun_compat (k j : nat) rho1 rho2 H1 H2 B1 e1 B2 e2 r1 r2
-          (IInvFunCompat :
-             forall H1 H1' H1''  H2  rho1 rho1' rho1'' rho2 env_loc, 
-               IIL1 (H1, rho1, Efun B1 e1) (H2, rho2, Efun B2 e2) ->
-               restrict_env (fundefs_fv B1) rho1 = rho1' ->
-               alloc (Env rho1') H1 = (env_loc, H1') ->
-               def_closures B1 B1 rho1 H1' env_loc = (H1'', rho1'') ->
-               IIL2 (H1'', rho1'', e1) (H2, def_funs B2 B2 rho2, e2)) :
+    Lemma cc_approx_exp_fun_compat (k j : nat) rho1 rho2 H1 H2 B1 e1 B2 e2 :
+      InvCtxCompat IL1 IL2 H1 H2 rho1 rho2 (Efun1_c B1 Hole_c) (Efun1_c B2 Hole_c) e1 e2 ->
+      IInvCtxCompat IIL1 IIL2 H1 H2 rho1 rho2 (Efun1_c B1 Hole_c) (Efun1_c B2 Hole_c) e1 e2 ->
+      InvCostBase IL1 IIL1 H1 H2 rho1 rho2 (Efun B1 e1) (Efun B2 e2) ->
 
       well_formed (reach' H1 (env_locs rho1 (occurs_free (Efun B1 e1)))) H1 ->
       (env_locs rho1 (occurs_free (Efun B1 e1))) \subset dom H1 ->
       
-
-      fundefs_num_fv B1 <= (r1 - r2) <= F*(cost H1 rho1 (Efun B1 e1)) -> 
-
       (forall H1 H1' H1'' rho1' rho_clo env_loc,
-
-         k >= cost H1 rho1 (Efun B1 e1) ->
 
          restrict_env (fundefs_fv B1) rho1 = rho_clo ->
          alloc (Env rho_clo) H1 = (env_loc, H1') ->
 
          def_closures B1 B1 rho1 H1' env_loc = (H1'', rho1') ->
 
-         (e1, rho1', H1'') ⪯ ^ (k - cost H1 rho1 (Efun B1 e1) ; j ; IIL2 ; IIG ; ILi r2 ; IG)
+         (e1, rho1', H1'') ⪯ ^ (k - cost (Efun B1 e1) ; j ; IIL2 ; IIG ; IL2 ; IG)
          (e2, def_funs B2 B2 rho2, H2)) ->
-      (Efun B1 e1, rho1, H1) ⪯ ^ (k ; j ; IIL1 ; IIG ; ILi r1 ; IG) (Efun B2 e2, rho2, H2).
+      
+      (Efun B1 e1, rho1, H1) ⪯ ^ (k ; j ; IIL1 ; IIG ; IL1 ; IG) (Efun B2 e2, rho2, H2).
     Proof with now eauto with Ensembles_DB.
-      intros Hwf Hdom Hleq Hpre b1 b2 H1' H2' rho1' rho2' v1 c1
+      intros Hinv Hiinv Hbase Hwf Hdom Hpre b1 b2 H1' H2' rho1' rho2' v1 c1
              m1 Heq1 Hinj1 Heq2 Hinj2 HII Hleq1 Hstep1 Hstuck1.
       inv Hstep1.
       (* Timeout! *)
-      - { simpl in Hcost. exists OOT, (c1 - r1).
+      - { simpl in Hcost. exists OOT, c1.
           - eexists. eexists id. repeat split. econstructor. simpl.
             omega. reflexivity.
             now eapply injective_subdomain_Empty_set.
-            eapply InvCostTimeout. eassumption.
+            eapply Hbase; eassumption.
             now rewrite cc_approx_val_eq. }
       (* Termination *)
       - { destruct (alloc (Env (restrict_env (fundefs_fv B1) rho1)) H1)
@@ -928,9 +1367,9 @@ Module Compat (H : Heap).
           - rewrite Hfuns, Hdef3 in Hs.
             destruct Hs as [Heq [Hfeq' [Hwf1 [Hwf2 [Henv1 [Henv2 Hinj]]]]]].
             edestruct Hpre as [v2 [c2 [m2 [b2' [Hstep [HS [Hinj' Hval]]]]]]]
-            ; [ | reflexivity | now apply Ha3 | now apply Hdef3 | |
+            ; [ | now apply Ha3 | now apply Hdef3 | |
                 | | | | | eassumption | | ].
-            + simpl in *; omega.
+            + reflexivity.
             + eapply heap_env_equiv_antimon. eassumption.
               normalize_occurs_free. rewrite <- Union_assoc. eapply Included_Union_preserv_r.
               eapply Included_Union_Setminus.
@@ -946,341 +1385,31 @@ Module Compat (H : Heap).
               eapply reach'_set_monotonic.
               eapply Included_trans. eapply def_funs_env_loc.
               eapply env_locs_monotonic. normalize_occurs_free...
-           + eapply IInvFunCompat; eauto.
+            + eapply Hiinv; try eassumption.
+              econstructor; eauto. now econstructor. 
+              econstructor; eauto. now econstructor.
            + simpl; omega.
-           + intros i. edestruct (Hstuck1 (i + cost H1' rho1' (Efun B1 e1))) as [r' [m' Hstep']].
+           + intros i. edestruct (Hstuck1 (i + cost (Efun B1 e1))) as [r' [m' Hstep']].
              inv Hstep'.
              * omega.
              * rewrite NPeano.Nat.add_sub in Hbs0. repeat subst_exp.
                repeat eexists. eassumption.
            + repeat eexists; eauto.
-             * eapply Eval_fun_per_cc with (c := c2 + cost H1' rho1' (Efun B2 e2)); try eassumption.
+             * eapply Eval_fun_per_cc with (c := c2 + cost (Efun B2 e2)); try eassumption.
                simpl. omega. reflexivity. simpl.
                rewrite NPeano.Nat.add_sub. eassumption.
-             * simpl. eapply InvCompat_str with (c2' := 1).
-               rewrite NPeano.Nat.add_sub. eassumption.
-               simpl. simpl in Hleq. omega. 
+             * simpl. eapply Hinv with (c2' := cost (Efun B2 e2)); try eassumption.
+               replace (c2 + 1 - cost (Efun B2 e2)) with c2 by (simpl; omega).
+               eassumption.
+               replace (cost (Efun B1 e1)) with (0 + cost_ctx (Efun1_c B1 Hole_c)) by (simpl; omega).
+               econstructor; eauto. now econstructor.
+               replace (cost (Efun B2 e2)) with (0 + cost_ctx (Efun1_c B2 Hole_c)) by (simpl; omega).
+               econstructor; eauto. now econstructor.
              * rewrite cc_approx_val_eq in *. 
                eapply cc_approx_val_monotonic. eassumption.
                simpl. simpl in Hcost. omega. }
-    Qed.
-    
-    Variable (clo_tag : cTag).
-    
-    Definition AppClo f t xs f' Γ :=
-      Eproj f' clo_tag 0%N f
-            (Eproj Γ clo_tag 1%N f
-                   (Eapp f' t (Γ :: xs))).
-
-    (* TODO move *)
-
-    (* Lemma heap_equiv_f_compose_r S (β1 β2 β3 β4 : loc -> loc) (H1 H2 H3 : heap block) : *)
-    (*   S |- H1 ≃_(β1, β2) H2 -> *)
-    (*   S |- H2 ≃_(β4 ∘ β2, β3) H3 -> *)
-    (*   S |- H1 ≃_(β4 ∘ β1, β3) H3. *)
-    (* Proof. *)
-    (* Admitted. *)
-
-   (* TODO move *)
-   Lemma live_deterministic S (_ : set_util.ToMSet S) H1 H2 H2' :
-      live S H1 H2 ->
-      live S H1 H2' ->
-      (exists b1 b2, S |- H2 ≃_(b1, b2) H2' /\
-                injective_subdomain (reach' H2 S) b1 /\
-                injective_subdomain (reach' H2' S) b2).
-   Proof.
-      intros [Hyp1 [b1 [Hyp2 Hinj1]]] [Hyp1' [b2 [Hyp2' Hinj2]]].
-      eexists b1, b2. symmetry in Hyp2. 
-      rewrite <- (Combinators.compose_id_right _ _ id) in Hyp2.
-      rewrite <- (Combinators.compose_id_left _ _ b2).
-      split; [| split ]; eauto.
-      eapply heap_equiv_f_compose; [| eassumption ]. eassumption.   
-   Qed.
-
-   (* Local invariants parameterized by the cost *)
-
-   Context (IIL1i : GIInv)
-           (IIL2i : GIInv)
-           (ILik : nat -> GInv). 
-
-    Context
-      (IL_heap_eq :
-         forall i k (H1 H2 H1' H2' : heap block) (rho1 rho2 rho1' rho2' : env) b1 b2 (e1 e2 : exp)
-           (c1 c2 m1 m2 : nat),
-         ILik k i (H1', rho1', e1, c1, m1) (H2', rho2', e2, c2, m2) ->
-         occurs_free e1 |- (H1, rho1) ⩪_( id, b1) (H1', rho1') ->
-         injective_subdomain (reach' H1' (env_locs rho1' (occurs_free e1))) b1 ->
-         occurs_free e2 |- (H2, rho2) ⩪_( b2, id) (H2', rho2') ->
-         injective_subdomain (reach' H2 (env_locs rho2 (occurs_free e2))) b2 ->
-         ILik k i (H1, rho1, e1, c1, m1) (H2, rho2, e2, c2, m2)).
-
-    Context
-      (IL1_mon :
-         forall i i' H1 rho1 e1 H2 rho2 e2,
-           IIL1i i (H1, rho1, e1) (H2, rho2, e2) ->
-           i' < i ->
-           IIL1i i' (H1, rho1, e1) (H2, rho2, e2)).
-    
-    Context
-      (IL2_mon :
-         forall i i' H1 rho1 e1 H2 rho2 e2,
-           IIL2i i (H1, rho1, e1) (H2, rho2, e2) ->
-           i' < i ->
-           IIL2i i' (H1, rho1, e1) (H2, rho2, e2)).
-
-    Context
-      (ILikCostTimeout :
-         forall i (H1 H2 : heap block) (rho1 rho2 : env) 
-           (e1 e2 : exp) (k c : nat),
-       IIL1i i (H1, rho1, e1) (H2, rho2, e2) ->
-       ILik k i (H1, rho1, e1, c, size_heap H1) (H2, rho2, e2, c - k, size_heap H2)).
-    
-    
-   (** Application compatibility *)
-   Lemma cc_approx_exp_app_compat (k j : nat) (b : Inj) (H1 H2 : heap block)
-          (rho1 rho2 : env) (f1 : var) (xs1 : list var)
-          (f2 f2' Γ : var) (xs2 : list var) (t : fTag) (c : nat)
-          (IInvAppCompat :
-             forall (i i' : nat) (H1 H2 H1' H1'' H2' : heap block) (rho1 rho_clo rho_clo1 rho_clo2 rho2 rho2' : env)
-               (B1 : fundefs) (f1 f1' : var) (ct1 : cTag) 
-               (xs1 xs1' : list var) (e1 : exp) (l1 env_loc1 : loc)
-               (vs1 : list value) 
-               (B2 : fundefs) (f2 f3 : var) (c ct2 : cTag) (xs2 xs2' : list var) 
-               (e2 : exp) (l2 env_loc2 : loc) (vs2 : list value),
-
-               IIL1i i (H1, rho1, Eapp f1 t xs1) (H2, rho2, AppClo f2 t xs2 f2' Γ) ->
-               i' < i ->
-               (* not exactly classy.... Can we make it a bit more abstract? *)
-               M.get f1 rho1 = Some (Loc l1) ->
-               get l1 H1 = Some (Clos (FunPtr B1 f1') (Loc env_loc1)) ->
-               get env_loc1 H1 = Some (Env rho_clo) ->
-               find_def f1' B1 = Some (ct1, xs1', e1) ->
-               getlist xs1 rho1 = Some vs1 ->
-               def_closures B1 B1 rho_clo H1 env_loc1 = (H1', rho_clo1) ->
-               setlist xs1' vs1 rho_clo1 = Some rho_clo2 ->
-               live (env_locs rho_clo2 (occurs_free e1)) H1' H1'' ->
-
-               M.get f2 rho2 = Some (Loc l2) ->
-               getlist xs2 rho2 = Some vs2 ->
-               get l2 H2 = Some (Constr c [FunPtr B2 f3; Loc env_loc2]) ->
-               Some rho2' =
-               setlist xs2' (Loc env_loc2 :: vs2) (def_funs B2 B2 (M.empty value)) ->
-               find_def f3 B2 = Some (ct2, xs2', e2) ->
-               live' (env_locs rho2' (occurs_free e2)) H2 H2' ->
-
-               (IIG i' (H1'', rho_clo2, e1) (H2', rho2', e2)) /\
-               (forall (k c1 c2 m1 m2 c1' c2' : nat),
-                  IG i' (H1', rho_clo2, e1, c1 - c1', m1) (H2, rho2', e2, c2 - c2', m2) ->
-                  c1' <= c2' + k <= c1' + F*c1' ->
-                  ILik k i (H1, rho1, Eapp f1 t xs1, c1, max m1 (size_heap H1'))
-                       (H2, rho2, AppClo f2 t xs2 f2' Γ, c2, max m2 (size_heap H2)))) :
-      
-      well_formed (reach' H1 (env_locs rho1 (occurs_free (Eapp f1 t xs1)))) H1 ->
-      well_formed (reach' H2 (env_locs rho2 (occurs_free (AppClo f2 t xs2 f2' Γ)))) H2 ->
-      (env_locs rho1 (occurs_free (Eapp f1 t xs1))) \subset dom H1 ->
-      (env_locs rho2 (occurs_free (AppClo f2 t xs2 f2' Γ))) \subset dom H2 ->
-      
-      ~ Γ \in (f2 |: FromList xs2) ->
-      ~ f2' \in (f2 |: FromList xs2) ->
-      Γ <> f2' ->
-
-      c + 3 <= F * (cost H1 rho1 (Eapp f1 t xs1)) -> 
-      length xs1 = length xs2 ->
-
-      cc_approx_var_env k j IIG IG b H1 rho1 H2 rho2 f1 f2 ->
-      Forall2 (cc_approx_var_env k j IIG IG b H1 rho1 H2 rho2) xs1 xs2 ->
-
-      (Eapp f1 t xs1, rho1, H1) ⪯ ^ (k ; j; IIL1i k ; IIG ; (fun p1 p2 => ILik c k (H1, rho1, Eapp f1 t xs1, fst p1, snd p1)
-                                                                            (H2, rho2, AppClo f2 t xs2 f2' Γ, fst p2, snd p2))
-                                                          ; IG) (AppClo f2 t xs2 f2' Γ, rho2, H2).
-   Proof with now eauto with Ensembles_DB.
-      intros Hwf1 Hwf2 Hs1 Hs2 Hnin1 Hnin2 Hneq Hleqc Hlen Hvar Hall
-             b1 b2 H1' H2' rho1' rho2' v1 c1 m1 Heq1 Hinj1 Heq2 Hinj2
-             HII Hleq1 Hstep1 Hstuck1.
-      eapply (cc_approx_var_env_heap_env_equiv
-                _ _ 
-                (occurs_free (Eapp f1 t xs1))
-                (occurs_free (AppClo f2 t xs2 f2' Γ))) in Hvar;
-          [| eassumption | eassumption | eassumption | eassumption 
-           | normalize_occurs_free; now eauto with Ensembles_DB
-           | unfold AppClo; normalize_occurs_free; now eauto with Ensembles_DB ].
-      inv Hstep1. 
-      (* Timeout! *)
-      - { edestruct (Hstuck1 (cost H1' rho1' (Eapp f1 t xs1))) as [v1 [m1 Hstep1]].
-          inv Hstep1; [ omega | ].
-          exists OOT, (c1 - c). destruct (lt_dec (c1 - c) 1).
-          - eexists. eexists id. repeat split. now constructor; eauto.
-            now eapply injective_subdomain_Empty_set. rewrite <- plus_n_O.
-            eapply IL_heap_eq; try eassumption.
-            eapply ILikCostTimeout. eassumption.
-            now rewrite cc_approx_val_eq.
-          - edestruct Hvar as [l2 [Hget' Hcc]]; eauto.
-            simpl in Hcc. rewrite Hgetl in Hcc. destruct l2 as [l2 | ]; [| contradiction ].
-            destruct (get l2 H2') as [v |] eqn:Hget2; try contradiction.
-            destruct Hcc as [Hbeq Hcc]; subst; simpl in Hcc.
-            destruct v as [ ? [| [| B2 f3 ] [| [ env_loc' |] [|] ]] | | ]; try contradiction.
-            destruct Hcc as [Him Hcc].
-            edestruct Hcc with (vs2 := vs) as (xs2' & e2 & rho2'' & Hfind' & Hset' & Hi'); try eassumption.
-            reflexivity. now firstorder. symmetry.
-            reflexivity. now firstorder.
-            destruct (lt_dec (c1 - c - 1) 1).
-            + eexists. eexists id. repeat split. unfold AppClo.
-              eapply Eval_proj_per_cc; eauto.
-              simpl. omega. reflexivity.
-              now econstructor; simpl; eauto.
-              eapply injective_subdomain_Empty_set.
-              rewrite <- !plus_n_O.
-              simpl. eapply IL_heap_eq; try eassumption.
-              eapply ILikCostTimeout. eassumption.
-              now rewrite cc_approx_val_eq.
-            + eexists. eexists id. repeat split. unfold AppClo.
-              eapply Eval_proj_per_cc; eauto.
-              simpl. omega. reflexivity.
-              eapply Eval_proj_per_cc; eauto.
-              simpl. omega.
-              rewrite M.gso. eassumption.
-              intros Heq; subst. now eauto with Ensembles_DB.
-              reflexivity. 
-              econstructor; try (now simpl; eauto). simpl.
-              erewrite <- Forall2_length; [| eassumption ]. simpl in *. omega.
-              now eapply injective_subdomain_Empty_set.
-              rewrite <- plus_n_O.
-              simpl. eapply IL_heap_eq; try eassumption.
-              eapply ILikCostTimeout. eassumption.
-              now rewrite cc_approx_val_eq. }
-      (* Termination *) 
-      - { simpl in Hcost.
-          eapply Forall2_monotonic_strong in Hall; (* yiiiiiikes *)
-            [| intros x1 x2 Hin1 Hin2 Hyp;
-               eapply (cc_approx_var_env_heap_env_equiv
-                         _ _
-                         (occurs_free (Eapp f1 t xs1))
-                         (occurs_free (AppClo f2 t xs2 f2' Γ))) in Hyp;
-               [ now eapply Hyp | eassumption | eassumption | eassumption | eassumption
-                 | normalize_occurs_free; now eauto with Ensembles_DB
-                 | unfold AppClo; repeat normalize_occurs_free; rewrite FromList_cons ];
-               right; constructor;
-               [ right; constructor;
-               [ now eauto with Ensembles_DB
-               | now intros Hc; inv Hc; eapply Hnin1; eauto ]
-               | now intros Hc; inv Hc; eapply Hnin2; eauto ] ].
-          edestruct (cc_approx_var_env_getlist IIG IG  k j rho1' rho2') as [vs2 [Hgetl' Hcc']];
-            [ eassumption | now eauto |].
-          edestruct Hvar as [l2 [Hget' Hcc]]; eauto.
-          simpl in Hcc. rewrite Hgetl in Hcc. destruct l2 as [l2 | ]; [| contradiction ]. 
-          destruct (get l2 H2') as [v |] eqn:Hget2; try contradiction.
-          destruct Hcc as [Hbeq Hcc]. simpl in Hcc.
-          destruct v as [ ? [| [| B2 f3 ] [| [ env_loc' |] [|] ]] | | ]; try contradiction.
-          edestruct Hcc as (Him & xs2' & e2 & rho2'' & Hfind' & Hset' & Hi'); try eassumption.
-          reflexivity. now firstorder. reflexivity. now firstorder.
-          edestruct (live_exists' (env_locs rho2'' (occurs_free e2)) H2') as [H2'' Hgc'].
-          assert (Hgc1 := Hgc); assert (Hgc2 := Hgc').
-          destruct Hgc as [Hseq [bgc [Heqgc Hinjgc]]].
-          destruct Hgc' as [Hseq' [bgc' [Heqgc' Hinjgc']]].
-          edestruct IInvAppCompat with (i' := k - cost H1' rho1' (Eapp f1 t xs1)) as [Hinv1 Hinv2]; try eassumption.
-          simpl. omega.
-          edestruct Hi' with (i := k - cost H1' rho1' (Eapp f1 t xs1))
-                               (j' := j) as [r2 [c2 [m2 [b2' [Hbs2 [Hinj [HIG Hcc2]]]]]]];
-            [ | omega | | | | | | | | | eassumption | | ].  
-          + simpl. omega.
-          + rewrite compose_id_neut_r. rewrite compose_id_neut_l. reflexivity.
-          + eapply Forall2_monotonic_strong; [| eassumption ].
-            intros v v' Hinv Hinv' Heq. rewrite cc_approx_val_eq.
-            eapply cc_approx_val_monotonic with (k := k).
-            assert (Hrv : val_loc v \subset env_locs rho1' (occurs_free (Eapp f1 t xs1))).
-            { normalize_occurs_free. rewrite env_locs_Union.
-              eapply Included_Union_preserv_l. rewrite env_locs_FromList.
-              simpl. eapply In_Union_list.
-              eapply in_map. eassumption. eassumption. }
-            assert (Hrv' : val_loc v' \subset env_locs rho2' (occurs_free (AppClo f2 t xs2 f2' Γ))).
-            { unfold AppClo. repeat normalize_occurs_free.
-              rewrite FromList_cons, !Setminus_Union_distr, !env_locs_Union.
-              do 2 eapply Included_Union_preserv_r.
-              eapply Included_Union_preserv_l. eapply Included_Union_preserv_r.
-              rewrite !Setminus_Disjoint.
-              rewrite env_locs_FromList.
-              simpl. eapply In_Union_list.
-              eapply in_map. eassumption. eassumption. 
-              now eapply Disjoint_Singleton_r; intros Hc; eapply Hnin1; eauto.
-              now eapply Disjoint_Singleton_r; intros Hc; inv Hc; eapply Hnin2; eauto. }
-            eapply cc_approx_val_heap_monotonic;
-              [ | | | | | now eapply HL.subheap_refl | ].
-            * eapply well_formed_respects_heap_env_equiv in Hwf1; [| eassumption ].
-              eapply well_formed_antimon; [| now apply Hwf1 ].
-              now eapply reach'_set_monotonic.
-            * eapply well_formed_respects_heap_env_equiv in Hwf2; [| eassumption ].
-              eapply well_formed_antimon; [| now apply Hwf2 ].
-              now eapply reach'_set_monotonic.
-            * eapply Included_trans; [| eapply reachable_in_dom; try eassumption ].
-              eapply Included_trans; [| now eapply reach'_extensive ].
-              eassumption.
-              eapply well_formed_respects_heap_env_equiv in Hwf1; [| eassumption ].
-              eassumption.
-              eapply env_locs_in_dom; eassumption.
-            * eapply Included_trans; [| eapply reachable_in_dom; try eassumption ].
-              eapply Included_trans; [| now eapply reach'_extensive ].
-              eassumption.
-              eapply well_formed_respects_heap_env_equiv in Hwf2; [| eassumption ].
-              eassumption.
-              eapply env_locs_in_dom; eassumption.
-            * eapply def_funs_subheap. eauto.
-            * eassumption.
-            * simpl; omega.
-          + eapply heap_env_equiv_heap_equiv. eassumption.
-          + eassumption.
-          + eapply heap_env_equiv_heap_equiv. eassumption.
-          + eassumption.
-          + eassumption.
-          + simpl; omega.
-          + intros i. edestruct (Hstuck1 (i + cost H1' rho1' (Eapp f1 t xs1))) as [r' [m' Hstep']].
-            inv Hstep'.
-            * omega.
-            * rewrite NPeano.Nat.add_sub in Hbs0.
-              repeat subst_exp. 
-              edestruct live_deterministic as [b1' [b2' [Heq [Hinj1' Hinj2']]]].
-              now apply Hgc1. now apply Hgc. try eassumption.
-              edestruct big_step_gc_heap_env_equiv_r
-                as [r1 [m1 [b1'' [b2''[Hgc'' _]]]]].
-              eassumption.
-              eapply heap_env_equiv_heap_equiv. symmetry. eassumption.
-              eassumption. eassumption. do 2 eexists. eassumption.
-          + do 3 eexists. exists b2'. repeat split.
-            * eapply Eval_proj_per_cc with
-              (c := c2 + 1 + 1 + cost H2' (M.set Γ (Loc env_loc') (M.set f2' (FunPtr B2 f3) rho2'))
-                                      (Eapp f2' t (Γ :: xs2))).
-              simpl; omega.
-              eassumption. eassumption. reflexivity.
-              eapply Eval_proj_per_cc. simpl; omega.
-              rewrite M.gso. eassumption.
-              intros Hc. subst. eapply Hnin2. now left; eauto.
-              eassumption. reflexivity. simpl.
-              eapply Eval_app_per_cc.
-              simpl. omega.
-              rewrite M.gso. rewrite M.gss. reflexivity.
-              now intros Hc; subst; eauto.
-              eassumption.
-              simpl. rewrite M.gss.
-              rewrite !getlist_set_neq. now rewrite Hgetl'.
-              intros Hc. eapply Hnin2. now eauto.
-              intros Hc. eapply Hnin1. now eauto.
-              now eauto. eassumption. reflexivity. simpl.
-              replace (c2 + 1 + 1 + S (S (length xs2)) - 1 - 1 - S (S (length xs2)))  with c2.
-              eassumption. omega.
-            * eassumption.
-            * simpl.
-              eapply IL_heap_eq; try eassumption.
-              eapply Hinv2 with
-              (c2' := 1 + 1 +
-                      cost H2' (M.set Γ (Loc env_loc') (M.set f2' (FunPtr B2 f3) rho2'))
-                           (Eapp f2' t (Γ :: xs2))).
-              simpl.
-              replace (c2 + 1 + 1 + S (S (length xs2)) - S (S (S (S (length xs2))))) with c2
-              by omega.
-              eassumption.
-              simpl in *. omega.
-            * rewrite cc_approx_val_eq in *. eapply cc_approx_val_monotonic.
-              eassumption. simpl. omega. }        
     Qed.    
+
    
     (* TODO move *)
     Lemma comp_ctx_f_Hole_c C :
@@ -1297,26 +1426,25 @@ Module Compat (H : Heap).
     Qed.
     
 
+    Context (ILC : exp_ctx -> Inv).
+    Context (IILC : exp_ctx -> IInv).
+(*
     Lemma cc_approx_exp_right_ctx_compat 
-          (k j : nat) rho1 rho2 rho2' H1 H2 H2' e1 C C' e2 c c' (II : exp_ctx -> IInv)
-          (IInvCtxCompat :
-             forall H1 H2 H2' rho1 rho2 rho2' e1 e2 C C' c, 
-               II C' (H1, rho1, e1) (H2, rho2, C |[ e2 ]|) ->
-               ctx_to_heap_env C H2 rho2 H2' rho2' c ->
-               II (comp_ctx_f C' C) (H1, rho1, e1) (H2', rho2', e2)) :
-
+          (k j : nat) rho1 rho2 rho2' H1 H2 H2' e1 C C' e2 c' :
+      InvCtxCompat_r (ILC C) (ILC C') H1 H2 rho1 rho2 C e1 e2 ->
+      IInvCtxCompat_r (IILC C) (IILC C') H1 H2 rho1 rho2 C e1 e2 ->
+      
       well_formed (reach' H1 (env_locs rho1 (occurs_free e1))) H1 ->
       well_formed (reach' H2 (env_locs rho2 (occurs_free (C |[ e2 ]|)))) H2 ->
       (env_locs rho1 (occurs_free e1)) \subset dom H1 ->
       (env_locs rho2 (occurs_free (C |[ e2 ]|))) \subset dom H2 ->
 
       ctx_to_heap_env C H2 rho2 H2' rho2' c' ->
-      (e1, rho1, H1) ⪯ ^ (k; j; II (comp_ctx_f C' C) ; IIG ; ILi (c' + c) ; IG) (e2, rho2', H2') ->
-      (e1, rho1, H1) ⪯ ^ (k; j; II C' ; IIG ; ILi c ; IG) (C |[ e2 ]|, rho2, H2).
+      (e1, rho1, H1) ⪯ ^ (k; j; IILC C' ; IIG ; ILC C' ; IG) (C' |[ e2 ]|, rho2', H2') ->
+      (e1, rho1, H1) ⪯ ^ (k; j; IILC (comp_ctx_f C C') ; IIG ; ILC (comp_ctx_f C C') ; IG) (C |[ C' |[ e2 ]| ]|, rho2, H2).
     Proof with now eauto with Ensembles_DB.
-      intros Hwf1 Hwf2 Henv1 Henv2 Hctx. revert c C'. induction Hctx; intros c1 C' Hpre.
-      - intros ? ? ? ? ? ? ? ? ? ? ? ? ? ? ? ? ?. eapply Hpre; eauto.
-        rewrite comp_ctx_f_Hole_c. eassumption.
+      intros Hinv Hiinv Hwf1 Hwf2 Henv1 Henv2 Hctx. induction Hctx; intros Hpre.
+      - simpl. eassumption.
       - rewrite <- plus_assoc in Hpre.
         replace (Econstr_c x t ys C) with (comp_ctx_f (Econstr_c x t ys Hole_c) C) in Hpre by reflexivity.
         rewrite <- comp_ctx_f_assoc with (c2 := Econstr_c x t ys Hole_c) in Hpre. 
@@ -1512,7 +1640,8 @@ Module Compat (H : Heap).
           eapply Included_trans; [| eassumption ].
           eapply env_locs_monotonic. simpl. normalize_occurs_free...
     Qed.
-    
-  End LR_Preds.
+    *)
+  End CompatLemmas.
+
   
 End Compat.
